Added a general "reverse b-bit fields" operation generalizing the existing "word_bytereverse", based on material from Juneyoung Lee. The operation also works on inputs where the word size is not an exact multiple of the field width, mapping bits in the upper overspill from b * N DIV b upwards to themselves, for definiteness. This is supported by an extension of BIT_WORD_CONV and WORD_RED_CONV as well as a custom conversion WORD_REVERSEFIELDS_CONV. Added a few more basic lemmas about this and other word concepts. New definition:
        word_reversefields

and theorems:

        BIT_WORD_REVERSEFIELDS
        VAL_WORD_AND_POW2_BITVAL
        WORD_AND_POW2_BITVAL
        WORD_BYTEREVERSE_REVERSEFIELDS
        WORD_REVERSEFIELDS_REVERSEFIELDS
        WORD_SHL_LSB
        WORD_SHL_LSB_ALT

Also updated NUM_DIV_CONV and NUM_MOD_CONV to handle the degenerate
cases of the form `m DIV 0` and `m MOD 0` (where m is a numeral),
which are fixed by definition to convenient values, 0 and m
respectively.

Library/words.ml
@@ -1742,6 +1742,30 @@ let VAL_WORD_AND_POW2 = prove
   COND_CASES_TAC THEN REWRITE_TAC[MULT_CLAUSES; LT_EXP; EXP_LT_0] THEN
   CONV_TAC NUM_REDUCE_CONV THEN ASM_MESON_TAC[BIT_TRIVIAL; NOT_LE]);;
 
+let WORD_AND_POW2_BITVAL = prove
+ (`(!(x:N word) k b.
+        word_and x (word(2 EXP k * bitval b)) =
+        word(2 EXP k * bitval(bit k x /\ b))) /\
+   (!(x:N word) k b.
+        word_and (word(2 EXP k * bitval b)) x =
+        word(2 EXP k * bitval(b /\ bit k x)))`,
+  REPEAT STRIP_TAC THEN BOOL_CASES_TAC `b:bool` THEN
+  ASM_REWRITE_TAC[BITVAL_CLAUSES; MULT_CLAUSES] THEN
+  REWRITE_TAC[WORD_AND_POW2; WORD_AND_EQ_0; BITS_OF_WORD_0] THEN
+  REWRITE_TAC[DISJOINT_EMPTY]);;
+
+let VAL_WORD_AND_POW2_BITVAL = prove
+ (`(!(x:N word) k b.
+        val(word_and x (word(2 EXP k * bitval b))) =
+        2 EXP k * bitval(bit k x /\ b)) /\
+   (!(x:N word) k b.
+        val(word_and (word(2 EXP k * bitval b)) x) =
+        2 EXP k * bitval(b /\ bit k x))`,
+  REPEAT STRIP_TAC THEN REWRITE_TAC[WORD_AND_POW2_BITVAL] THEN
+  MATCH_MP_TAC VAL_WORD_EQ THEN REWRITE_TAC[bitval] THEN
+  COND_CASES_TAC THEN REWRITE_TAC[MULT_CLAUSES; LT_EXP; EXP_LT_0] THEN
+  CONV_TAC NUM_REDUCE_CONV THEN ASM_MESON_TAC[BIT_TRIVIAL; NOT_LE]);;
+
 let VAL_WORD_AND_LE = prove
  (`(!x y:N word. val(word_and x y) <= val x) /\
    (!x y:N word. val(word_and x y) <= val y)`,
@@ -2339,6 +2363,22 @@ let WORD_SHL_COMPOSE = prove
   REPEAT GEN_TAC THEN REWRITE_TAC[word_shl; VAL_WORD; EXP_ADD] THEN
   REWRITE_TAC[WORD_EQ; CONG] THEN CONV_TAC MOD_DOWN_CONV THEN
   REWRITE_TAC[MULT_ASSOC]);;
+
+let WORD_SHL_LSB_ALT = prove
+ (`!x:N word.
+        word_shl x (dimindex(:N) - 1) =
+        if bit 0 x then word(2 EXP (dimindex(:N) - 1)) else word 0`,
+  GEN_TAC THEN COND_CASES_TAC THEN
+  REWRITE_TAC[WORD_EQ_BITS_ALT; BIT_WORD_0; BIT_WORD_POW2; BIT_WORD_SHL] THEN
+  X_GEN_TAC `i:num` THEN ASM_CASES_TAC `i = dimindex(:N) - 1` THEN
+  ASM_REWRITE_TAC[SUB_REFL] THEN ASM_ARITH_TAC);;
+
+let WORD_SHL_LSB = prove
+ (`!x:N word.
+        word_shl x (dimindex(:N) - 1) =
+        word(2 EXP (dimindex(:N) - 1) * bitval(bit 0 x))`,
+  GEN_TAC THEN REWRITE_TAC[WORD_SHL_LSB_ALT; bitval] THEN
+  COND_CASES_TAC THEN ASM_REWRITE_TAC[MULT_CLAUSES]);;
 
 let word_ushr = new_definition
   `word_ushr (x:(N)word) n =
@@ -4737,6 +4777,58 @@ let WORD_CLZ_MONO = prove
   REWRITE_TAC[WORD_LE_CLZ_VAL] THEN ASM_ARITH_TAC);;
 
 (* ------------------------------------------------------------------------- *)
+(* Reversal of the b-bit fields in an N-bit word. If N isn't a multiple      *)
+(* of b, this leaves bits above the highest b multiple unchanged.            *)
+(* ------------------------------------------------------------------------- *)
+
+let word_reversefields = new_definition
+ `(word_reversefields:num->(N)word->(N)word) (b:num) w =
+  word_of_bits
+    { i | i < dimindex(:N) /\
+          bit (if i < b * dimindex(:N) DIV b
+               then b * (dimindex(:N) DIV b - 1 - i DIV b) + i MOD b
+               else i) w}`;;
+
+let BIT_WORD_REVERSEFIELDS = prove
+ (`!(x:(N)word) b i.
+        bit i (word_reversefields b x) <=>
+        i < dimindex(:N) /\
+        bit (if i < b * dimindex(:N) DIV b
+             then b * (dimindex(:N) DIV b - 1 - i DIV b) + i MOD b
+             else i) x`,
+  REPEAT GEN_TAC THEN REWRITE_TAC[word_reversefields; BIT_WORD_OF_BITS] THEN
+  REWRITE_TAC[IN_ELIM_THM] THEN MESON_TAC[]);;
+
+let WORD_REVERSEFIELDS_REVERSEFIELDS = prove
+ (`!(x:(N)word) b. word_reversefields b (word_reversefields b x) = x`,
+  ONCE_REWRITE_TAC[WORD_EQ_BITS_ALT] THEN
+  REWRITE_TAC[BIT_WORD_REVERSEFIELDS] THEN
+  REPEAT STRIP_TAC THEN ASM_REWRITE_TAC[] THEN
+  DISJ_CASES_TAC(ARITH_RULE `b = 0 \/ 0 < b`) THEN
+  ASM_REWRITE_TAC[MOD_ZERO; DIV_ZERO; MULT_CLAUSES; ADD_CLAUSES; LT] THEN
+  ABBREV_TAC `q = dimindex (:N) DIV b` THEN
+  ASM_CASES_TAC `i:num < b * q` THEN ASM_REWRITE_TAC[] THEN
+  ASM_SIMP_TAC[ONCE_REWRITE_RULE[MULT_SYM] DIV_MULT; LE_1; DIV_MULT_ADD;
+    MOD_MULT_ADD; MOD_MOD_REFL; DIV_LT; MOD_LT_EQ_LT; ADD_CLAUSES] THEN
+  SUBGOAL_THEN `b * (q - 1 - i DIV b) + i MOD b < b * q` ASSUME_TAC THENL
+   [MATCH_MP_TAC(ARITH_RULE
+     `m < n /\ n * (x + 1) <= n * q ==> n * x + m < n * q`) THEN
+    ASM_REWRITE_TAC[MOD_LT_EQ_LT; LE_MULT_LCANCEL] THEN
+    UNDISCH_TAC `i < b * q` THEN
+    ASM_CASES_TAC `q = 0` THEN ASM_REWRITE_TAC[] THEN ASM_ARITH_TAC;
+    ASM_REWRITE_TAC[]] THEN
+  MATCH_MP_TAC(TAUT `p /\ (q <=> q') ==> (p /\ q <=> q')`) THEN CONJ_TAC THENL
+   [TRANS_TAC LTE_TRANS `b * q:num` THEN ASM_REWRITE_TAC[] THEN
+    MP_TAC(SPECL [`dimindex(:N)`; `b:num`] DIVISION) THEN
+    ASM_REWRITE_TAC[] THEN ASM_ARITH_TAC;
+    AP_THM_TAC THEN AP_TERM_TAC THEN
+    TRANS_TAC EQ_TRANS `b * i DIV b + i MOD b` THEN
+    CONJ_TAC THENL [ALL_TAC; REWRITE_TAC[DIVISION_SIMP]] THEN
+    AP_THM_TAC THEN AP_TERM_TAC THEN AP_TERM_TAC THEN
+    MATCH_MP_TAC(ARITH_RULE `x < n ==> n - 1 - (n - 1 - x) = x`) THEN
+    ASM_SIMP_TAC[RDIV_LT_EQ; LE_1] THEN ASM_ARITH_TAC]);;
+
+(* ------------------------------------------------------------------------- *)
 (* Byte reversal, with type constrained to multiple of 8.                    *)
 (* ------------------------------------------------------------------------- *)
 
@@ -4766,6 +4858,14 @@ let WORD_BYTEREVERSE_BYTEREVERSE = prove
   AP_THM_TAC THEN AP_TERM_TAC THEN
   SIMP_TAC[MOD_MULT_ADD; MOD_MOD_REFL; DIV_MULT_ADD; ARITH_EQ] THEN
   SIMP_TAC[DIV_LT; MOD_LT_EQ; ARITH_EQ] THEN ASM_ARITH_TAC);;
+
+let WORD_BYTEREVERSE_REVERSEFIELDS = prove
+ (`word_bytereverse = word_reversefields 8`,
+  REWRITE_TAC[FUN_EQ_THM] THEN GEN_TAC THEN
+  GEN_REWRITE_TAC I [WORD_EQ_BITS_ALT] THEN
+  REWRITE_TAC[BIT_WORD_BYTEREVERSE; BIT_WORD_REVERSEFIELDS] THEN
+  REWRITE_TAC[DIMINDEX_TYBIT0; MULT_ASSOC] THEN
+  CONV_TAC NUM_REDUCE_CONV THEN SIMP_TAC[DIV_MULT; ARITH_EQ]);;
 
 (* ------------------------------------------------------------------------- *)
 (* Alignment. The definition rolls in the assumption that the value is a     *)
@@ -5336,6 +5436,15 @@ let BIT_WORD_CONV =
         BINOP2_CONV (DEPTH_CONV((!word_SIZE_CONV) ORELSEC NUM_RED_CONV))
          (LAND_CONV (DEPTH_CONV((!word_SIZE_CONV) ORELSEC NUM_RED_CONV))) THENC
         (conv_and_t ORELSEC conv_and_f)) tm
+
+    | Comb(Comb(Const("bit",_),n),
+           Comb(Comb(Const("word_reversefields",_),b),_))
+      when is_numeral n && is_numeral b ->
+       (GEN_REWRITE_CONV I [BIT_WORD_REVERSEFIELDS] THENC
+        BINOP2_CONV (DEPTH_CONV((!word_SIZE_CONV) ORELSEC NUM_RED_CONV))
+         (LAND_CONV (DEPTH_CONV((!word_SIZE_CONV) ORELSEC NUM_RED_CONV))) THENC
+        (conv_and_t ORELSEC conv_and_f)) tm
+
     | _ -> failwith "BIT_WORD_CONV";;
 
 (* ------------------------------------------------------------------------- *)
@@ -6304,6 +6413,38 @@ let WORD_BYTEREVERSE_CONV =
   RAND_CONV EXPAND_NSUM_CONV THENC
   DEPTH_CONV(GEN_REWRITE_CONV I [BITVAL_CLAUSES] ORELSEC NUM_RED_CONV);;
 
+let WORD_REVERSEFIELDS_CONV =
+  let pth = (SPECL [`NUMERAL b`; `NUMERAL n`] o prove)
+   (`!b n.
+        word_reversefields b (word n:N word) =
+        word(nsum (0..dimindex(:N)-1)
+          (\i. 2 EXP i *
+               bitval(ODD(n DIV
+               2 EXP (if i < b * dimindex(:N) DIV b
+                      then b * (dimindex(:N) DIV b - 1 - i DIV b) + i MOD b
+                      else i)))))`,
+    REPEAT GEN_TAC THEN GEN_REWRITE_TAC I [WORD_EQ_BITS_ALT] THEN
+    REWRITE_TAC[BIT_WORD_REVERSEFIELDS; BIT_WORD] THEN
+    X_GEN_TAC `i:num` THEN DISCH_TAC THEN ASM_REWRITE_TAC[] THEN
+    MATCH_MP_TAC(TAUT `p /\ (q <=> q') ==> (p /\ q <=> q')`) THEN
+    CONJ_TAC THENL
+     [ASM_CASES_TAC `b = 0` THEN ASM_REWRITE_TAC[MULT_CLAUSES; LT] THEN
+      ASM_CASES_TAC `dimindex (:N) DIV b = 0` THEN
+      ASM_REWRITE_TAC[MULT_CLAUSES; LT] THEN
+      COND_CASES_TAC THEN ASM_REWRITE_TAC[] THEN
+      MATCH_MP_TAC(ARITH_RULE
+       `b * (x + 1) <= n /\ m < b ==> b * x + m < n`) THEN
+      ASM_SIMP_TAC[MOD_LT_EQ; GSYM LDIV_LT_EQ] THEN ASM_ARITH_TAC;
+      GEN_REWRITE_TAC RAND_CONV [ODD_MOD] THEN
+      SIMP_TAC[DIGITSUM_DIV_MOD; FINITE_NUMSEG; BITVAL_BOUND_ALT] THEN
+      ASM_SIMP_TAC[IN_NUMSEG; LE_0; ARITH_RULE `i < n ==> i <= n - 1`] THEN
+      REWRITE_TAC[BITVAL_EQ_1]]) in
+  GEN_REWRITE_CONV I [pth] THENC
+  DEPTH_CONV
+   ((!word_SIZE_CONV) ORELSEC NUM_MULT_CONV ORELSEC NUM_SUB_CONV) THENC
+  RAND_CONV EXPAND_NSUM_CONV THENC
+  DEPTH_CONV(GEN_REWRITE_CONV I [BITVAL_CLAUSES] ORELSEC NUM_RED_CONV);;
+
 let WORD_JSHL_CONV =
   let pth = prove
    (`word_jshl (word(NUMERAL m):N word) (word(NUMERAL n):N word) =
@@ -6430,6 +6571,8 @@ let WORD_RED_CONV =
     `word_clz (word(NUMERAL n):N word)`,WORD_CLZ_CONV;
     `word_bytereverse (word(NUMERAL n):((((N)tybit0)tybit0)tybit0)word)`,
                 WORD_BYTEREVERSE_CONV;
+    `word_reversefields (NUMERAL b) (word(NUMERAL n):N word)`,
+                WORD_REVERSEFIELDS_CONV;
     `word_jshl (word(NUMERAL m):N word) (word(NUMERAL n))`,WORD_JSHL_CONV;
     `word_jshr (word(NUMERAL m):N word) (word(NUMERAL n))`,WORD_JSHR_CONV;
     `word_jushr (word(NUMERAL m):N word) (word(NUMERAL n))`,WORD_JUSHR_CONV;
